\documentclass[12pt, a4paper]{article}
\setlength{\parindent}{0pt}
\usepackage[a4paper, portrait, margin=1in]{geometry}
\usepackage{preamble}

\newtheorem*{theorem}{Theorem}

\newcommand{\F}{\mathbb{F}}
\newcommand{\im}{\operatorname{im}}

\begin{document}
\textbf{(Q3)}
\begin{proof}
    The "column $j$" expansion of $\det A$ can be rewritten as:
    \[
        \sum_{j = 1}^n (-1)^{j + i} A_{ji} \det(\tilde{A}_{ji})
    \]

    We then use the fact that $\det A = \det A^t$.

    The cofactor (row $i$)expansion of $\det A^t$ is given as:
    \[
        \sum_{j = 1}^{n} (-1)^{i + j} A^{t}_{ij} \det (\tilde{A^t}_{ij})
        =
        \sum_{j = 1}^{n} (-1)^{i + j} A_{ji} \det (\tilde{A}_{ji})
    \]
    by the definition of $A^t$.
\end{proof}
\end{document}