\documentclass[12pt, a4paper]{article}
\setlength{\parindent}{0pt}
\usepackage[a4paper, portrait, margin=1in]{geometry}
\usepackage{preamble}

\newtheorem*{theorem}{Theorem}

\newcommand{\F}{\mathbb{F}}

\begin{document}
\textbf{(Q7)}

\textit{(a)}

\begin{align*}
    (3 + 2i)z & = (2 + i)(-2i)\\
    (3 + 2i)z & = 2 - 4i\\
    z & = (2 - 4i) \cdot \frac{3 -2i}{3^2 + 2^2} = \frac{-(2 + 16i)}{13}
\end{align*}

\textit{(b)}

\begin{gather*}
    z^6  = -125\\
    z^6 = 125e^{i(\pi + 2k\pi)}\\
    z  = \sqrt[6]{125}e^{i\frac{\pi}{6} + \frac{2k\pi}{6}}\\
    z  = x + yi \st  x = \sqrt{5} \cos \left(\frac{\pi}{6} + \frac{2k\pi}{6}\right)\\
    y = \sqrt{5} \sin \left(\frac{\pi}{6} + \frac{2k\pi}{6}\right)\\
    \Downarrow\\
    x = \sqrt{5}\cos(\frac{3\pi}{6}), \sqrt{5}\cos(\frac{5\pi}{6}),
    \ldots, \sqrt{5}\cos(\frac{13\pi}{6})\\
    = 0, \frac{\sqrt{15}}{2}, \frac{\sqrt{15}}{2}, 0, \frac{\sqrt{15}}{2},
    \frac{\sqrt{15}}{2}\\
    y = \sqrt{5}\sin(\frac{3\pi}{6}), \sqrt{5}\sin(\frac{5\pi}{6}),
    \ldots, \sqrt{5}\sin(\frac{13\pi}{6})\\
    y = \sqrt{5}, \pm\frac{\sqrt{5}}{2}, -\sqrt{5}, \mp\frac{\sqrt{5}}{2}\\
    \Downarrow\\
    z = \pm\sqrt{5}i, \frac{\sqrt{15}}{2} \pm \frac{\sqrt{5}}{2}
\end{gather*}

\textit{(c)}

\begin{gather*}
    e^z = 1 - \sqrt{3}i\\
    e^x e^iy = \sqrt{1 + 3}e^{i\frac{\pi}{3}} = 2e^{i\frac{\pi}{3}}\\
    \therefore e^x = 2 \implies x = \ln 2, y = -\frac{\pi}{3}\\
    \therefore z = \ln 2 - \frac{\pi}{3}i
\end{gather*}

\end{document}