\documentclass[12pt, a4paper]{article}
\setlength{\parindent}{0pt}
\usepackage[a4paper, portrait, margin=1in]{geometry}
\usepackage{preamble}

\newtheorem*{theorem}{Theorem}

\newcommand{\F}{\mathbb{F}}
\newcommand{\Om}{\operatorname{O}}

\begin{document}
\textbf{(Q2)}

\textit{(a)}
\begin{proof}
    First assume $[A, B] = O_n$. Then $AB - BA = \textbf{O}_n \implies AB = BA$.

    Then assume $AB = BA$. Then by definition, $[A, B] = AB - BA = \textbf{O}_n$.
\end{proof}

\textit{(b)}
\begin{proof}
    By definition, $[B, A] = BA - AB$. Then

    \[
        -(BA - AB) = -[B, A] = (AB - BA) = [A, B]
    \]
\end{proof}

\textit{(c)}
\begin{proof}
    By definition of $[A, B]$, we expand the given expressions:
    \begin{align*}
        [A, [B, C]] & = [A, (BC - CB)] = A(BC - CB) = (BC - CB)A\\
        & = ABC - ACB - BCA + CBA\\
        [C, [A, B]] & = [C, (AB - BA)] = C(AB - BA) - (AB - BA)C\\
        & = CAB - CBA - ABC + BAC\\
        [B, [C, A]] & = [B, (CA - AC)] = B(CA - AC) - (CA - AC)B\\
        & = BCA - BAC - CAB + ACB
    \end{align*}

    Adding all 3 expanded expressions together, we see that we can
    form pairs of matrix products and their negatives:

    \begin{align*}
          & (ABC - ABC) + (ACB - ACB)\\
        + & (BAC - BAC) + (BCA - BCA)\\
        + & (CAB - CAB) + (CBA - CBA)\\
        = & \Om_{n \times n}
    \end{align*}
\end{proof}
\end{document}