\documentclass[12pt, a4paper]{article}
\setlength{\parindent}{0pt}
\usepackage[a4paper, portrait, margin=1in]{geometry}
\usepackage{preamble}

\newtheorem*{theorem}{Theorem}

\newcommand{\F}{\mathbb{F}}

\begin{document}

\textbf{(Q11)}

\begin{proof}
    Let $S$ be a basis for $W_1 \cap W_2$, where
    $S = \{u_1, u_2, \ldots u_r\}$ and $\dim (W_1 \cap W_2) = r$.

    Let $B_1$ be a basis of $W_1$ and $B_2$ be a basis of $W_2$.
    By the Replacement Theorem, since $(W_1 \cap W_2) \sse W_1$ and $\sse W_2$,
    we can express $B_1$ and $B_2$ as follows:

    \begin{gather*}
        B_1 = \{u_1, u_2, \ldots, v_1, \ldots v_s\} \implies \dim W_1 = r + s\\
        B_2 = \{u_1, u_2, \ldots, w_1, \ldots w_t\} \implies \dim W_2 = r + t\\
    \end{gather*}

    Let $B = B_1 \cup B_2$. Then

    \[
        B = \{u_1, u_2, \ldots v_1, \ldots v_s, w_1, \ldots w_t\}
    \]

    Since $|B| = (r + s) + (r + t) - r = \dim W_1 + \dim W_2 - \dim (W_1 \cap W_@)$,
    it now remains to prove that $B$ is a basis for $V$.

    To show linear independence, let

    \[
        \sum_{i = 1}^{r} a_i u_i +
        \sum_{j = 1}^{s} b_j v_j +
        \sum_{k = 1}^{t} c_k w_k = 0
    \]

    Since $u_i$ and $v_j$ form $B_1$ we can conclude that
    $a, b = 0 \;\; \forall i, j$.

    Similarly, since $u_i, w_k$ for $B_2$, we can conclude the same for
    $b, c \;\; \forall i, j$.

    We now prove that $B$ spans $W_1 + W_2$. Let $w \in (W_1 + W_2)$.
    Then $w = w_1 + w_2$ where $w_1 \in W_1, w_2 \in W_2$.

    Then
    \begin{gather*}
        w_1 = \sum_{i = 1}^{r} p_i u_i + \sum_{j = 1}^{s} q_j v_j\\
        w_2 = \sum_{i = 1}^{r} g_i u_i + \sum_{k = 1}^{t} h_k w_k\\
        w = \sum_{i = 1}^{r} (p_i + g_i)u_i + \sum_{j = 1}^{s} q_j v_j
        + \sum_{k = 1}^{t} h_k w_k
    \end{gather*}

    Which is in $\operatorname{span} B$.

\end{proof}

\end{document}